case_study/MinimalCaps/Contracts.v
@@ -226,7 +226,7 @@ Module MinCapsSymbolicContractKit <:
   Definition sep_contract_write_mem : SepContract ["c" ∶ ty_cap, "v" ∶ ty_memval ] ty_unit :=
     {| sep_contract_logic_variables := ["c" ∶ ty_cap, "v" ∶ ty_memval];
        sep_contract_localstore      := [term_var "c", term_var "v"]%arg;
-       sep_contract_precondition    := asn_csafe (term_var "c");
+       sep_contract_precondition    := asn_safe (term_var "v") ✱ asn_csafe (term_var "c");
        sep_contract_result          := "write_mem_result";
        sep_contract_postcondition   :=
          asn_csafe (term_var "c") ✱ asn_eq (term_var "write_mem_result") (term_lit ty_unit tt);
@@ -650,16 +650,16 @@ Module MinCapsSymbolicContractKit <:
     {| sep_contract_logic_variables := ["address" ∶ ty_addr, "new_value" ∶ ty_memval, "p" ∶ ty_perm, "b" ∶ ty_addr, "e" ∶ ty_addr];
        sep_contract_localstore      := [term_var "address", term_var "new_value"]%arg;
        sep_contract_precondition    :=
-         asn_csafe (term_record capability
-                            [term_var "p",
-                             term_var "b",
-                             term_var "e",
-                             term_var "address"]) ✱
-                        (asn_match_enum permission (term_var "p")
-                            (fun p => match p with
-                                    | RW => asn_within_bounds (term_var "address") (term_var "b") (term_var "e")
-                                    | _  => asn_false
-                                    end));
+         asn_safe (term_var "new_value") ✱ asn_csafe (term_record capability
+                                                                  [term_var "p",
+                                                                   term_var "b",
+                                                                   term_var "e",
+                                                                   term_var "address"])
+                  ✱ (asn_match_enum permission (term_var "p")
+                                    (fun p => match p with
+                                           | RW => asn_within_bounds (term_var "address") (term_var "b") (term_var "e")
+                                           | _  => asn_false
+                                           end));
        sep_contract_result          := "wM_result";
        sep_contract_postcondition   :=
          asn_csafe (term_record capability
